Experimenting with HOLCF + quotient_definition

Denotational.thy
@@ -1,5 +1,5 @@
 theory Denotational
-  imports Terms Heap "FMap-HOLCF" "FMap-Nominal" "~~/src/HOL/HOLCF/Library/Option_Cpo" "~~/src/HOL/HOLCF/HOLCF"  
+  imports Terms Heap "FMap-HOLCF" "FMap-Nominal" "~~/src/HOL/HOLCF/Library/Option_Cpo" "~~/src/HOL/HOLCF/HOLCF"
 begin
 
 default_sort cpo
@@ -14,6 +14,14 @@ class cont_pt =
   cpo + 
   pt +
   assumes perm_cont: "\<And>p. cont ((permute p) :: 'a::{cpo,pt} \<Rightarrow> 'a)"
+
+class discr_pt = 
+  discrete_cpo + 
+  pt
+
+instance discr_pt \<subseteq> cont_pt
+ by (default, auto)
+
 
 lemma (in cont_pt) perm_cont_simp[simp]: "\<pi> \<bullet> x \<sqsubseteq> \<pi> \<bullet> y \<longleftrightarrow> x \<sqsubseteq> y"
   apply rule
@@ -138,6 +146,11 @@ begin
   done
 end
 
+lemma permute_cfun_eq: "permute p = (\<lambda> f. (Abs_cfun (permute p)) oo f oo (Abs_cfun (permute (-p))))"
+  by (rule, rule cfun_eqI, auto simp add: permute_cfun_def)
+
+instance "cfun" :: (cont_pt, cont_pt) cont_pt
+  by (default,subst permute_cfun_eq, auto)
 
 lemma Lam_eqvt:
   "cont f \<Longrightarrow> \<pi> \<bullet> Abs_cfun f = Abs_cfun (\<pi> \<bullet> f)"
@@ -228,7 +241,7 @@ translations
 
 
 lemma cfun_upd_eqvt[eqvt]: "p \<bullet> (cfun_upd f (x::'a::{cont_pt,discrete_cpo}) y) = cfun_upd (p \<bullet> f) (p \<bullet> x) (p \<bullet> y)"
-  by (auto simp add:permute_cfun_def cfun_eq_iff cfun_upd_def)
+  apply (auto simp add:permute_cfun_def cfun_eq_iff cfun_upd_def) done
 
 domain Value = Fn (lazy "Value \<rightarrow> Value")
 
@@ -272,12 +285,12 @@ lemma heapToEnv_eqvt[eqvt]:
 lemma heapToEnv_fdom[simp]:"fdom (heapToEnv h eval) = fst ` set h"
   by (induct h eval rule:heapToEnv.induct, auto)
 
-definition heapExtend :: "Env \<Rightarrow> heap \<Rightarrow> (Env \<Rightarrow> exp \<Rightarrow> Value)  \<Rightarrow> (var, Value) fmap"
+definition heapExtend :: "Env \<Rightarrow> heap \<Rightarrow> (exp \<Rightarrow> Env \<Rightarrow> Value)  \<Rightarrow> (var, Value) fmap"
   where
-  "heapExtend \<rho> h eval = fmap_update \<rho> (fix1 (fmap_bottom (fst ` set h))  (\<Lambda> \<rho>'. heapToEnv h (eval \<rho>')))"
+  "heapExtend \<rho> h eval = fmap_update \<rho> (fix1 (fmap_bottom (fst ` set h))  (\<Lambda> \<rho>'. heapToEnv h (\<lambda> e. eval e \<rho>')))"
 
 lemma heapExtend_eqvt:
-  "(\<And>e. cont (\<lambda>\<rho>. eval \<rho> e)) \<Longrightarrow> \<pi> \<bullet> heapExtend \<rho> h eval = heapExtend (\<pi> \<bullet> \<rho>) (\<pi> \<bullet> h) (\<pi> \<bullet> eval)"
+  "(\<And>e. cont (eval e)) \<Longrightarrow> \<pi> \<bullet> heapExtend \<rho> h eval = heapExtend (\<pi> \<bullet> \<rho>) (\<pi> \<bullet> h) (\<pi> \<bullet> eval)"
 unfolding heapExtend_def
   apply (subst fmap_update_eqvt)
   apply (subst fix1_eqvt)
@@ -295,7 +308,7 @@ where
 | "\<lbrakk> App e x \<rbrakk>\<^bsub>\<rho>\<^esub> = \<lbrakk> e \<rbrakk>\<^bsub>\<rho>\<^esub> \<down>Fn \<lbrakk> Var x \<rbrakk>\<^bsub>\<rho>\<^esub> "
 | "\<lbrakk> Var x \<rbrakk>\<^bsub>\<rho>\<^esub> = the (lookup \<rho> x)"
 | "set (bn as) \<sharp>* \<rho> \<Longrightarrow>\<lbrakk> Let as body\<rbrakk>\<^bsub>\<rho>\<^esub> = \<lbrakk> Let as body\<rbrakk>\<^bsub>\<lbrace> asToHeap as \<rbrace>\<rho>\<^esub>"
-| "\<lbrace> h \<rbrace>\<rho> = heapExtend \<rho> h (\<lambda> \<rho>' e . \<lbrakk>e\<rbrakk>\<^bsub>\<rho>'\<^esub>)"
+| "\<lbrace> h \<rbrace>\<rho> = heapExtend \<rho> h ESem"
 proof-
 have eqvt_at_ESem: "\<And> a b . eqvt_at ESem_HSem_sumC (Inl (a, b)) \<Longrightarrow> eqvt_at (\<lambda>(a, b). ESem a b) (a, b)" sorry
 have eqvt_at_HSem: "\<And> a b . eqvt_at ESem_HSem_sumC (Inr (a, b)) \<Longrightarrow> eqvt_at (\<lambda>(a, b). HSem a b) (a, b)" sorry
@@ -414,5 +427,251 @@ case (goal16 as \<rho> body as' \<rho>' body')
     qed
 }
 qed auto
+
+instantiation exp :: discrete_cpo
+begin
+  definition  [simp]: "(x::exp) \<sqsubseteq> y \<longleftrightarrow> x = y"
+  instance by default simp
+end
+
+instantiation exp_raw :: discr_pt
+begin
+  definition  [simp]: "(x::exp_raw) \<sqsubseteq> y \<longleftrightarrow> x = y"
+  instance by default simp
+end
+
+instantiation assn_raw :: discrete_cpo
+begin
+  definition  [simp]: "(x::assn_raw) \<sqsubseteq> y \<longleftrightarrow> x = y"
+  instance by default simp
+end
+
+
+(*
+find_theorems (100) name:exp name:"split"
+
+definition
+  match_Lam :: "exp \<rightarrow> (var \<rightarrow> exp \<rightarrow> 'b match) \<rightarrow> 'b match"
+where
+  "match_Lam = (\<Lambda> e k. case e of (Lam [x]. e) \<Rightarrow> k x e | _ \<Rightarrow>  Fixrec.fail)"
+
+lemma match_Lam_simps [simp]:
+  "match_Lam\<cdot>(Lam [x]. e)\<cdot>k = k\<cdot>x\<cdot>e"
+  "match_Lam\<cdot>(Var x)\<cdot>k = Fixrec.fail"
+unfolding match_Lam_def by simp_all
+
+setup {*
+  Fixrec.add_matchers
+    [ (@{const_name Lam}, @{const_name match_Lam})) ]
+*}
+*)
+
+definition
+  match_Lam_raw :: "exp_raw \<rightarrow> (var \<rightarrow> exp_raw \<rightarrow> 'b match) \<rightarrow> 'b match"
+where
+  "match_Lam_raw = (\<Lambda> e k. case e of (Lam_raw x e) \<Rightarrow> k \<cdot> x \<cdot> e | _ \<Rightarrow>  Fixrec.fail)"
+
+definition
+  match_App_raw :: "exp_raw \<rightarrow> (exp_raw \<rightarrow> var \<rightarrow> 'b match) \<rightarrow> 'b match"
+where
+  "match_App_raw = (\<Lambda> e k. case e of (App_raw e v) \<Rightarrow> k \<cdot> e \<cdot> v | _ \<Rightarrow>  Fixrec.fail)"
+
+definition
+  match_Var_raw :: "exp_raw \<rightarrow> ( var \<rightarrow> 'b match) \<rightarrow> 'b match"
+where
+  "match_Var_raw = (\<Lambda> e k. case e of (Var_raw v) \<Rightarrow> k \<cdot> v | _ \<Rightarrow>  Fixrec.fail)"
+
+definition
+  match_Let_raw :: "exp_raw \<rightarrow> (assn_raw \<rightarrow> exp_raw \<rightarrow> 'b match) \<rightarrow> 'b match"
+where
+  "match_Let_raw = (\<Lambda> e k. case e of (Let_raw as e) \<Rightarrow> k \<cdot> as \<cdot> e | _ \<Rightarrow>  Fixrec.fail)"
+
+setup {*
+  Fixrec.add_matchers
+    [ (@{const_name Lam_raw}, @{const_name match_Lam_raw})
+    , (@{const_name App_raw}, @{const_name match_App_raw})
+    , (@{const_name Var_raw}, @{const_name match_Var_raw})
+    , (@{const_name Let_raw}, @{const_name match_Let_raw})
+    ]
+*}
+
+lemma match_Lam_raw_simps [simp]:
+  "match_Lam_raw\<cdot>(Lam_raw x e)\<cdot>k = k\<cdot>x\<cdot>e"
+  "match_Lam_raw\<cdot>(App_raw e x)\<cdot>k = Fixrec.fail"
+  "match_Lam_raw\<cdot>(Var_raw x)\<cdot>k = Fixrec.fail"
+  "match_Lam_raw\<cdot>(Let_raw as e)\<cdot>k = Fixrec.fail"
+unfolding match_Lam_raw_def by simp_all
+
+lemma match_App_raw_simps [simp]:
+  "match_App_raw\<cdot>(Lam_raw x e)\<cdot>k = Fixrec.fail"
+  "match_App_raw\<cdot>(App_raw e x)\<cdot>k = k\<cdot>e\<cdot>x"
+  "match_App_raw\<cdot>(Var_raw x)\<cdot>k = Fixrec.fail"
+  "match_App_raw\<cdot>(Let_raw as e)\<cdot>k = Fixrec.fail"
+unfolding match_App_raw_def by simp_all
+
+lemma match_Var_raw_simps [simp]:
+  "match_Var_raw\<cdot>(Lam_raw x e)\<cdot>k = Fixrec.fail"
+  "match_Var_raw\<cdot>(App_raw e x)\<cdot>k = Fixrec.fail"
+  "match_Var_raw\<cdot>(Var_raw x)\<cdot>k = k\<cdot>x"
+  "match_Var_raw\<cdot>(Let_raw as e)\<cdot>k = Fixrec.fail"
+unfolding match_Var_raw_def by simp_all
+
+lemma match_Let_raw_simps [simp]:
+  "match_Let_raw\<cdot>(Lam_raw x e)\<cdot>k = Fixrec.fail"
+  "match_Let_raw\<cdot>(App_raw e x)\<cdot>k = Fixrec.fail"
+  "match_Let_raw\<cdot>(Var_raw x)\<cdot>k = Fixrec.fail"
+  "match_Let_raw\<cdot>(Let_raw as e)\<cdot>k = k\<cdot>as\<cdot>e"
+unfolding match_Let_raw_def by simp_all
+
+lemma cont2cont_lookup[simp,cont2cont]:
+  "cont f \<Longrightarrow> cont (\<lambda>p. the (lookup (f p) x))" sorry
+
+function heapToEnv_raw :: "(var \<times> exp_raw) list \<Rightarrow> (exp_raw \<Rightarrow> Value) \<Rightarrow> Env"
+where
+  "heapToEnv_raw [] _ = fempty"
+| "heapToEnv_raw ((x,e)#h) eval = (heapToEnv_raw h eval) (x f\<mapsto> eval e)"
+by (pat_completeness, auto)
+termination by lexicographic_order
+
+lemma cont2cont_heapToEnv_raw[simp, cont2cont]:
+  "(\<And> e. cont (\<lambda>\<rho>. eval \<rho> e)) \<Longrightarrow> cont (\<lambda> \<rho>. heapToEnv_raw h (eval \<rho>))"
+  by(induct h, auto)
+
+lemma heapToEnv_raw_eqvt[eqvt]:
+  "\<pi> \<bullet> heapToEnv_raw h eval = heapToEnv_raw (\<pi> \<bullet> h) (\<pi> \<bullet> eval)"
+  by (induct h eval rule:heapToEnv_raw.induct, auto simp add: fmap_upd_eqvt  permute_fun_def)
+
+lemma heapToEnv_raw_fdom[simp]:"fdom (heapToEnv_raw h eval) = fst ` set h"
+  by (induct h eval rule:heapToEnv_raw.induct, auto)
+
+
+definition heapExtend_raw :: "Env \<Rightarrow> (var \<times> exp_raw) list \<Rightarrow> (exp_raw \<rightarrow> Env \<rightarrow> Value)  \<Rightarrow> (var, Value) fmap"
+  where
+  "heapExtend_raw \<rho> h eval = fmap_update \<rho> (fix1 (fmap_bottom (fst ` set h))  (\<Lambda> \<rho>'. heapToEnv_raw h (\<lambda> e. eval\<cdot>e\<cdot>\<rho>')))"
+
+lemma heapExtend_raw_eqvt:
+  "\<pi> \<bullet> heapExtend_raw \<rho> h eval = heapExtend_raw (\<pi> \<bullet> \<rho>) (\<pi> \<bullet> h) (\<pi> \<bullet> eval)"
+unfolding heapExtend_raw_def
+  apply (subst fmap_update_eqvt)
+  apply (subst fix1_eqvt)
+  apply (auto intro: fmap_belowI' simp add: fmap_bottom_eqvt  Lam_eqvt)
+  apply perm_simp
+  apply rule
+  done
+
+lemma cont2cont_heapExtend_raw[simp,cont2cont]:
+  "cont f \<Longrightarrow> cont g \<Longrightarrow> cont(\<lambda> x. heapExtend_raw (f x) h (g x))" sorry
+
+lemma cont2cont_heapExtend[simp,cont2cont]:
+  "cont f \<Longrightarrow> cont g \<Longrightarrow> cont(\<lambda> x. heapExtend (f x) h (g x))" sorry
+
+lemma cont2cont_rep_exp[simp,cont2cont]:
+  "cont f \<Longrightarrow> cont(\<lambda> x. rep_exp (f x))" sorry
+
+
+fixrec
+  ESem2 :: "exp_raw \<rightarrow> (Env \<rightarrow> Value)" 
+where
+  "atom x \<sharp> \<rho> \<Longrightarrow> ESem2\<cdot>(Lam_raw x e) \<cdot> \<rho> = Fn \<cdot> (\<Lambda> v. (ESem2 \<cdot> e \<cdot> (\<rho>(x f\<mapsto> v))))"
+| "ESem2\<cdot>(App_raw e x) \<cdot> \<rho> = (ESem2 \<cdot> e \<cdot> \<rho>) \<down>Fn (ESem2 \<cdot> (Var_raw x) \<cdot> \<rho>) "
+| "ESem2\<cdot>(Var_raw x) \<cdot> \<rho> = the (lookup \<rho> x)"
+| "ESem2\<cdot>(Let_raw as body) \<cdot> \<rho> =  ESem2 \<cdot> body \<cdot> (heapExtend_raw \<rho> (asToHeap_raw as) ESem2)"
+
+definition map_cfun :: "('c \<Rightarrow> 'a) \<Rightarrow> ('b \<Rightarrow> 'd) \<Rightarrow> ('a \<rightarrow> 'b) \<Rightarrow> ('c \<rightarrow> 'd)" where
+  "map_cfun f g h = (\<Lambda> x. g (h \<cdot> (f x)))"
+
+definition
+  cfun_rel :: "('a \<Rightarrow> 'c \<Rightarrow> bool) \<Rightarrow> ('b \<Rightarrow> 'd \<Rightarrow> bool) \<Rightarrow> ('a \<rightarrow> 'b) \<Rightarrow> ('c \<rightarrow> 'd) \<Rightarrow> bool" (infixr "\<cdot>===>" 55)
+where
+  "cfun_rel A B = (\<lambda>f g. \<forall>x y. A x y \<longrightarrow> B (f\<cdot>x) (g\<cdot>y))"
+
+lemma cfun_quotient3:
+  assumes q1: "Quotient3 R1 abs1 rep1"
+  and     q2: "Quotient3 R2 abs2 rep2"
+  shows "Quotient3 (R1 \<cdot>===> R2) (map_cfun rep1 abs2) (map_cfun abs1 rep2)"
+  sorry
+
+declare [[mapQ3 "cfun" = (cfun_rel, cfun_quotient3)]]
+
+definition map_fmap :: "('c \<Rightarrow> 'a) \<Rightarrow> ('b \<Rightarrow> 'd) \<Rightarrow> ('a, 'b) fmap \<Rightarrow> ('c, 'd) fmap" where
+  "map_fmap f g h = undefined"
+
+definition
+  fmap_rel :: "('a \<Rightarrow> 'c \<Rightarrow> bool) \<Rightarrow> ('b \<Rightarrow> 'd \<Rightarrow> bool) \<Rightarrow> ('a, 'b) fmap \<Rightarrow> ('c, 'd) fmap \<Rightarrow> bool" (infixr "f===>" 55)
+where
+  "fmap_rel A B = (\<lambda>f g. undefined)"
+
+lemma fmap_quotient3:
+  assumes q1: "Quotient3 R1 abs1 rep1"
+  and     q2: "Quotient3 R2 abs2 rep2"
+  shows "Quotient3 (R1 f===> R2) (map_fmap rep1 abs2) (map_fmap abs1 rep2)"
+  sorry
+
+declare [[mapQ3 "fmap" = (fmap_rel, fmap_quotient3)]]
+
+
+definition 
+  match_rel :: "('a \<Rightarrow> 'b \<Rightarrow> bool) \<Rightarrow> 'a match \<Rightarrow> 'b match \<Rightarrow> bool"
+where
+  "match_rel R a b = undefined"
+
+lemma [simp]: "match_rel (op =) = op =" sorry
+
+definition
+  map_match :: "('a \<Rightarrow> 'b) \<Rightarrow> 'a match \<Rightarrow> 'b match"
+where
+  "map_match = undefined"
+
+lemma match_quotient [quot_thm]:
+  assumes "Quotient3 R Abs Rep"
+  shows "Quotient3 (match_rel R) (map_match Abs) (map_match Rep)"
+  sorry
+declare [[mapQ3 "match" = (match_rel, match_quotient)]]
+
+(*
+Cannot allow the Nominal constructors in HOLCF as a match_Lam would not
+be equivariant (as the continuation might not be)
+
+quotient_definition
+  "match_Lam :: exp \<rightarrow> (var \<rightarrow> exp \<rightarrow> 'b match) \<rightarrow> 'b match"
+  is "match_Lam_raw"
+unfolding cfun_rel_def
+apply auto
+thm alpha_exp_raw.cases
+apply (erule alpha_exp_raw.cases)
+unfolding match_Lam_raw_def
+apply auto
+*)
+
+quotient_definition  "ESem3 :: exp \<rightarrow> Env \<rightarrow> Value" is ESem2
+unfolding cfun_rel_def
+find_theorems alpha_exp_raw
+apply rule
+apply rule
+apply rule
+apply (rule cfun_eqI)
+
+apply (induct rule:ESem2.induct)
+apply auto
+
+apply (erule alpha_exp_raw.cases)
+apply auto
+
+defer
+apply (rule cfun_eqI, simp)
+
+
+
+oops
+
+(*
+find_theorems ESem2
+apply (induct rule:ESem2.induct)
+find_theorems name:alpha_exp_raw
+apply auto
+apply (erule alpha_exp_raw_alpha_assn_raw_alpha_bn_raw.inducts)
+apply auto
+*)
+
 
 end
